README.md
@@ -4,4 +4,6 @@ A replication in __lean 4__ of some of the __scala__ code used in the _PolyMath 
 
 This fork of the repository is an attempt to understand and experiment with the approach of producing computer-generated proofs for length bounds on words in a free group.
 
+It contains a formalisation of the result from the paper [Random words in free groups, non-crossing matches and RNA secondary structures](https://arxiv.org/pdf/2007.12109.pdf), concerning the minimality of a certain length function known as the "Watson-Crick length". 
+
 ---
